Verify that i2c_state_rel is preserved after a clock cycle
Signed-off-by: Liam Murphy <liampm32@gmail.com>

common/cheshireOracleScript.sml
@@ -58,4 +58,47 @@ Definition cheshire_oracle_def:
     (cheshire_oracle_write eat_fnum tick write)
 End
 
+(* Performs either a device memory read, write, or no-op from a Cheshire
+ * peripheral model. *)
+Definition cheshire_req_def:
+  cheshire_req
+    (read_fn: 'ffi -> num -> num -> ffi_outcome + 'notif option # word32)
+    (write_fn: 'ffi -> num -> num -> word32 -> ffi_outcome + ('ffi -> 'ffi) # 'notif option)
+    (st: 'ffi) (valid: bool) (write: bool) (nb: num) (offset: num) (wdata: word32) =
+  if ~valid then
+    INR (I, NONE, NONE)
+  else if write then
+    SUM_MAP I (\(st_upd, notif). (st_upd, notif, NONE)) (write_fn st nb offset wdata)
+  else
+    SUM_MAP I (\(notif, rdata). (I, notif, SOME rdata)) (read_fn st nb offset)
+End
+
+Theorem cheshire_req_INR_cases:
+  cheshire_req read_fn write_fn st valid write nb offset wdata = INR (st_upd, notif, rdata) ==>
+  (~valid /\ st_upd = I /\ notif = NONE /\ rdata = NONE) \/
+  (valid /\ ~write /\ st_upd = I /\ (?value. rdata = SOME value /\ read_fn st nb offset = INR (notif, value))) \/
+  (valid /\ write /\ rdata = NONE /\ write_fn st nb offset wdata = INR (st_upd, notif))
+Proof
+  Cases_on `valid`
+  >- (Cases_on `write`
+      >- (Cases_on `write_fn st nb offset wdata`
+          >- simp [cheshire_req_def]
+          >- (Cases_on `y` >> simp [cheshire_req_def]))
+      >- (Cases_on `read_fn st nb offset`
+          >- simp [cheshire_req_def]
+          >- (Cases_on `y` >> simp [cheshire_req_def])))
+  >- simp [cheshire_req_def]
+QED
+
+Theorem cheshire_req_INR_st_upd_cases:
+  cheshire_req read_fn write_fn st valid write nb offset wdata = INR (st_upd, notif, rdata) ==>
+  (~(valid /\ write) /\ st_upd = I) \/
+  (valid /\ write /\ write_fn st nb offset wdata = INR (st_upd, notif))
+Proof
+  rpt strip_tac
+  >> dxrule cheshire_req_INR_cases
+  >> rpt strip_tac
+  >> simp []
+QED
+
 val _ = export_theory ();
