i2c/i2cCircuitCompileScript.sml
@@ -1,0 +1,49 @@
+open HolKernel Parse boolLib bossLib;
+open translatorLib verilogPrintLib;
+open i2cRegsCircuitLib;
+open i2cCircuitTheory;
+
+val _ = new_theory "i2cCircuitCompile";
+
+local
+  val outputs = [
+    "reg_rsp_o",
+
+    "cio_scl_o",
+    "cio_scl_en_o",
+    "cio_sda_o",
+    "cio_sda_en_o",
+
+    "intr_fmt_threshold_o",
+    "intr_rx_threshold_o",
+    "intr_fmt_overflow_o",
+    "intr_rx_overflow_o",
+    "intr_nak_o",
+    "intr_scl_interference_o",
+    "intr_sda_interference_o",
+    "intr_stretch_timeout_o",
+    "intr_sda_unstable_o",
+    "intr_cmd_complete_o",
+    "intr_tx_stretch_o",
+    "intr_tx_overflow_o",
+    "intr_acq_full_o",
+    "intr_unexp_stop_o",
+    "intr_host_timeout_o"
+  ];
+  val comms = i2c_reg_comms @ [];
+in
+  val tstate = init_translator i2c_circuit_def [] comms;
+  val trans_thm = module2hardware tstate i2c_circuit_def [] outputs comms;
+end
+
+val verilogstr =
+  definition "i2c_circuit_v_def"
+  |> REWRITE_RULE [definition "i2c_circuit_v_seqs_def", definition "i2c_circuit_v_combs_def", definition "i2c_circuit_v_decls_def"]
+  |> concl
+  |> rhs
+  |> verilog_print "i2c_circuit" "clk_i" (SOME "rst_ni");
+
+val f = TextIO.openOut "i2c_circuit.sv";
+val _ = output (f, verilogstr);
+
+val _ = export_theory ();
