i2c/i2cCircuitScript.sml
@@ -1,5 +1,5 @@
 open HolKernel Parse boolLib bossLib;
-open translatorLib verilogPrintLib;
+open translatorLib;
 open i2cRegsCircuitLib;
 open cheshireCircuitTheory i2cCircuitStateTheory;
 
@@ -17,7 +17,7 @@ Definition i2c_reg_top_ff_def:
   i2c_reg_top_ff (fext: i2c_circuit_ext_state) (s: i2c_circuit_state) (s': i2c_circuit_state) = ^i2c_reg_top_ff_tm
 End
 
-Theorem i2c_reg_top_comb_1_trans = SIMP_RULE (pure_ss ++ ARITH_ss) [reg_req_decode_def, reg_req_accfupds, combinTheory.K_THM, dimindex_7] i2c_reg_top_comb_1_def;
+Theorem i2c_reg_top_comb_1_trans = SIMP_RULE (pure_ss ++ ARITH_ss) [reg_req_decode_def, reg_req_accfupds, combinTheory.K_THM, wordsTheory.dimindex_7] i2c_reg_top_comb_1_def;
 
 val init_tm = add_x_inits ``
   <|
@@ -33,46 +33,5 @@ End
 Definition i2c_circuit_def:
   i2c_circuit = mk_module (procs [i2c_reg_top_ff]) (procs [i2c_reg_top_comb_1; i2c_reg_top_comb_2]) i2c_circuit_init
 End
-
-local
-  val outputs = [
-    "reg_rsp_o",
-
-    "cio_scl_o",
-    "cio_scl_en_o",
-    "cio_sda_o",
-    "cio_sda_en_o",
-
-    "intr_fmt_threshold_o",
-    "intr_rx_threshold_o",
-    "intr_fmt_overflow_o",
-    "intr_rx_overflow_o",
-    "intr_nak_o",
-    "intr_scl_interference_o",
-    "intr_sda_interference_o",
-    "intr_stretch_timeout_o",
-    "intr_sda_unstable_o",
-    "intr_cmd_complete_o",
-    "intr_tx_stretch_o",
-    "intr_tx_overflow_o",
-    "intr_acq_full_o",
-    "intr_unexp_stop_o",
-    "intr_host_timeout_o"
-  ];
-  val comms = i2c_reg_comms @ [];
-in
-  val tstate = init_translator i2c_circuit_def [] comms;
-  val trans_thm = module2hardware tstate i2c_circuit_def [] outputs comms;
-end
-
-val verilogstr =
-  definition "i2c_circuit_v_def"
-  |> REWRITE_RULE [definition "i2c_circuit_v_seqs_def", definition "i2c_circuit_v_combs_def", definition "i2c_circuit_v_decls_def"]
-  |> concl
-  |> rhs
-  |> verilog_print "i2c_circuit" "clk_i" (SOME "rst_ni");
-
-val f = TextIO.openOut "i2c_circuit.sv";
-val _ = output (f, verilogstr);
 
 val _ = export_theory ();
